Note about missing stuff in Get spec;
Need to know that when the latestEpoch is increased, the value that is
initially set for the new per-epoch value is the value that used to be
in latestEpoch. This will allow the caller to know that the new epoch is
going to start out in sync with the end-client (epoch-unaware) points-to.

src/program_proof/fencing/frontend_proof.v
@@ -11,6 +11,31 @@ Context `{!heapGS Σ}.
 Local Definition q2 := (1/2)%Qp.
 Local Definition q4 := (1/4)%Qp.
 
+Definition k0 := (U64 0).
+Definition k1 := (U64 1).
+
+Definition kv_ptsto (k v:u64) : iProp Σ.
+Admitted.
+
+Global Instance kv_ptsto_timeless k v : Timeless (kv_ptsto k v).
+Admitted.
+
+Definition is_mepoch_lb (e:u64) : iProp Σ.
+Admitted.
+
+Definition own_mepoch (e:u64) : iProp Σ.
+Admitted.
+
+Global Instance own_mepoch_timeless e : Timeless (own_mepoch e).
+Admitted.
+
+Definition frontend_inv_def: iProp Σ :=
+  ∃ (latestEpoch v:u64),
+  "HlatestEpoch" ∷ own_epoch latestEpoch q2 ∗
+  "HlatestMEpoch" ∷ own_mepoch latestEpoch ∗
+  "Hval" ∷ own_val latestEpoch (Some v) q4 ∗
+  "Hkv" ∷ kv_ptsto k0 v.
+
 Definition own_Server (s:loc) (epoch:u64) : iProp Σ :=
   ∃ (ck1 ck2:loc),
   "#Hepoch" ∷ readonly (s ↦[frontend.Server :: "epoch"] #epoch) ∗
@@ -19,8 +44,7 @@ Definition own_Server (s:loc) (epoch:u64) : iProp Σ :=
   "Hck1_own" ∷ own_Clerk ck1 ∗
   "Hck2_own" ∷ own_Clerk ck2 ∗
 
-  "Hghost1" ∷ (∃ ov, own_val epoch ov q4) ∗
-  (* either have 1/2, or have 1/4 and have witness that latestEpoch >= epoch *)
+  "Hghost1" ∷ (∃ ov, own_val epoch ov q2 ∨ is_mepoch_lb epoch ∗ own_val epoch ov q4) ∗
   (* TODO: add second value *)
   "_" ∷ True.
 
@@ -31,22 +55,6 @@ Definition is_Server s : iProp Σ :=
   "Hmu" ∷ readonly (s ↦[frontend.Server :: "mu"] mu) ∗
   "HmuInv" ∷ is_lock frontendN mu (∃ epoch, own_Server s epoch)
 .
-
-Definition k0 := (U64 0).
-Definition k1 := (U64 1).
-
-Definition kv_ptsto (k v:u64) : iProp Σ.
-Admitted.
-
-Global Instance kv_ptsto_timeless k v : Timeless (kv_ptsto k v).
-Admitted.
-
-Definition frontend_inv_def: iProp Σ :=
-  ∃ (latestEpoch v:u64),
-  "HlatestEpoch" ∷ own_epoch latestEpoch q2 ∗
-  "Hval" ∷ own_val latestEpoch (Some v) q4 ∗
-  "Hkv" ∷ kv_ptsto k0 v.
-
 Definition frontend_inv : iProp Σ :=
   inv frontendN (frontend_inv_def).
 
@@ -84,9 +92,15 @@ Proof.
     iInv "Hinv" as ">Hown" "Hclose".
     iNamed "Hown".
     iModIntro.
-    iExists _; iFrame.
+    iExists _; iFrame "HlatestEpoch".
     iIntros "%Hfresh HlatestEpoch".
     iModIntro.
+    iAssert (∃ oldv, own_val epoch oldv (1/2))%I with "[Hghost1]" as (?) "HH".
+    {
+      admit.
+    }
+    iExists _; iFrame "HH".
+    (* TODO: Get() spec needs to say something about new value *)
     admit.
   }
 Admitted.
